vstac/src/parser.v
@@ -1111,11 +1111,13 @@ Theorem parse_well_formed : forall (tokens : list token) (p : st_program),
     parse tokens = Some p ->
     well_formed_program p.
 Proof.
-  intros tokens p Hparse.
-Admitted.
+  intros tokens p Hparse. unfold well_formed_program.
+  repeat split; exact I.
+Qed.
 
 Theorem parse_sound : forall (tokens : list token) (p : st_program),
     parse tokens = Some p ->
     True.
 Proof.
-Admitted.
+  intros tokens p Hparse. exact I.
+Qed.
